newLibrary/countQuery.dfy
@@ -1,0 +1,65 @@
+include "verifiableLucid.dfy"
+
+/*  A simple example that uses verifiable lucid to 
+    implement a simple program with a counting packet forwarder 
+    and a control-plane query event that returns the count of packets.
+    This program uses single handler verification. */
+
+module CountQuery refines VerifiableLucid {
+
+    // Events
+    datatype Event = 
+        | pkt(src : uint32, dst : uint32)
+        | getCount(i : uint32)
+        | countReport(i : uint32, count : uint32)
+
+    class Program ... {
+        // Array and initialization
+        var pktCtr : LArray<uint32>
+
+        constructor () 
+            ensures fresh(pktCtr)
+            ensures fresh(this)
+            ensures pktCtr.cells == seq(8, (_ => 0))
+        {   
+            pktCtr := new LArray<uint32>.Create(8, 0);            
+        }
+
+        // Memops
+        function incr (oldVal: uint32, incrBy: uint32) : uint32 { 
+            to_uint32(oldVal + incrBy) 
+        }
+        function memval (oldVal: uint32, unused: uint32) : uint32 { oldVal }
+
+        // Packet handler specification: 
+        //                1. pkt emits packets with source 0 to port 0, 
+        //                   and all other packets to port 1.
+        //                2. pkt increments pktCtr[src % 8] by 1.
+        method Pkt(src : uint32, dst : uint32) 
+            modifies    this`emittedEvents, this.pktCtr`cells    
+            requires |pktCtr.cells| == 8 
+            ensures         ((src == 0) ==> emits(0, pkt(src, dst)))
+                        &&  ((src != 0) ==> emits(1, pkt(src, dst)))
+            ensures  LArray.updated_cell(pktCtr, src % 8, (old(pktCtr.cells)[src % 8] + 1) % max32)
+        {
+            if (src == 0) {
+                generate_port(0, pkt(src, dst));
+            } else {
+                generate_port(1, pkt(src, dst));
+            }
+            LArray<uint32>.Set(pktCtr, src % 8, incr, 1);
+        }
+
+        // count query specification
+        // getCount emits a countReport event with the count of packets in pktCtr[i % 8].
+        method getCount(i : uint32)
+            modifies this`emittedEvents
+            requires |pktCtr.cells| == 8 
+            ensures emits(0, countReport(i, old(pktCtr.cells)[i % 8]))
+        {
+            var count := LArray<uint32>.Get(pktCtr, i % 8, memval, 0);
+            generate_port(0, countReport(i, count));
+        }        
+    }
+}
+
