newLibrary/recircCount.dfy
@@ -1,0 +1,59 @@
+include "verifiableLucid.dfy"
+
+/* A program that counts on recirculation. */
+
+module RecircCount refines VerifiableLucid {
+
+    // Events
+    datatype Event = 
+        | pkt(src : uint32, dst : uint32)
+        | count(i : uint32)
+
+    class Program ... {
+        // Array and initialization
+        var pktCtr : LArray<uint32>
+
+        constructor () 
+            ensures fresh(pktCtr)
+            ensures fresh(this)
+            ensures pktCtr.cells == seq(8, (_ => 0))
+        {   
+            pktCtr := new LArray<uint32>.Create(8, 0);            
+        }
+
+        // Memops
+        function incr (oldVal: uint32, incrBy: uint32) : uint32 { 
+            to_uint32(oldVal + incrBy)
+        }
+        function memval (oldVal: uint32, unused: uint32) : uint32 { oldVal }
+
+        // Packet handler specification: 
+        //                1. pkt emits packets with source 0 to port 0, 
+        //                   and all other packets to port 1.
+        //                2. pkt increments pktCtr[src % 8] by 1.
+        method Pkt(src : uint32, dst : uint32) 
+            modifies    this`emittedEvents, this`generatedEvent
+            requires readyToHandle(pkt(src, dst))
+            ensures src == 0 ==> emits(0, pkt(src, dst))
+            ensures src != 0 ==> emits(1, pkt(src, dst))
+            ensures generates(count(src))
+        {
+            if (src == 0) {
+                generate_port(0, pkt(src, dst));
+            } else {
+                generate_port(1, pkt(src, dst));
+            }
+            generate(count(src));
+        }
+        // Count increments pktCtr[i % 8], and only pktCtr[i % 8], by 1.
+        method Count(i : uint32)
+            modifies pktCtr`cells
+            requires |pktCtr.cells| == 8 
+            ensures  LArray.updated_cell(pktCtr, i % 8, (old(pktCtr.cells)[i % 8] + 1) % max32)
+        {
+            var count := LArray<uint32>.Get(pktCtr, i % 8, memval, 0);
+            LArray<uint32>.Set(pktCtr, i % 8, incr, 1);
+        }        
+    }
+}
+
